examples/sbf/main_theorem.v
@@ -10,34 +10,138 @@ Require Import ProD3.examples.sbf.switch.
 Require Import ProD3.examples.sbf.flow_proof.
 Require Import ProD3.examples.sbf.verif_switch.
 
-Check process_packet_fw_process_packet.
+Definition abs_flow_wf (ps : list Packet) : Prop :=
+  forall i : Z, 0 <= i < Zlength ps ->
+  0 <= fst (snd (fst (Znth i ps))) < Z.pow 2 32
+    /\ 0 <= snd (snd (fst (Znth i ps))) < Z.pow 2 32.
 
 Lemma process_packets_trans_fw : forall es f ps es' rs,
   filter_repr f es ->
+  abs_flow_wf ps ->
   process_packets ge P4_types.metadata_t es ps es' rs ->
   exists f',
     filter_repr f' es' /\ trans_fw f ps f' rs.
-Admitted.
+Proof.
+  intros es f ps; revert es f; induction ps as [ | p ps ?]; intros.
+  - inv H1.
+    eexists; split; eauto. constructor.
+  - inv H1.
+    assert (abs_flow_wf ps). {
+      clear -H0. unfold abs_flow_wf in *.
+      intros. specialize (H0 (i + 1) ltac:(list_solve)).
+      replace (Znth (i + 1) (p :: ps)) with (Znth i ps) in * by list_solve.
+      lia.
+    }
+    assert (H2 : 0 <= fst (snd (fst p)) < Z.pow 2 32 /\ 0 <= snd (snd (fst p)) < Z.pow 2 32). {
+      clear -H0. unfold abs_flow_wf in *.
+      specialize (H0 0 ltac:(list_solve)).
+      list_solve.
+    }
+    destruct H2.
+    eapply process_packet_fw_process_packet in H5; only 2-4 : eassumption.
+    destruct H5 as [f' []].
+    specialize (IHps _ _ _ _ ltac:(eassumption) ltac:(eassumption) ltac:(eassumption)).
+    destruct IHps as [? []].
+    eexists; split; eauto.
+    eapply trans_cons; eauto.
+Qed.
 
 Lemma high_level_exec_trans_fw_iff : forall h p res,
   high_level_exec h p res <->
   exists h' f,
     trans_fw (empty (get_tstamp (Znth 0 (h++[p])))) (h ++ [p]) f
     (h' ++ [res]).
-Admitted.
+Proof.
+  intros; split; intros.
+  - destruct H as [? [? [? []]]].
+    repeat eexists; econstructor; eauto.
+  - destruct H as [? [? H]].
+    eapply trans_app_inv in H. 2 : auto.
+    destruct H as [? [? [? [? []]]]].
+    eapply trans_cons_inv in H0. 2 : auto.
+    destruct H0 as [? [? [? [? []]]]].
+    inv H2. 2 : { clear -H4. list_solve. }
+    replace res with x5. 2 : {
+      clear -H1.
+      pose (Inhabitant_Result := (res : Inhabitant Result)).
+      assert (Znth (Zlength x) (x ++ [res]) = (Znth (Zlength x) (x2 ++ [x5]))) by congruence.
+      list_solve.
+    }
+    repeat eexists; eauto.
+Qed.
 
 Definition init_es := ltac:(get_init_es am_ge p4ast.prog).
 
+Definition filter_empty := @ConFilter.filter_empty num_frames num_rows num_slots H_num_frames H_num_rows H_num_slots.
+
+Ltac simpl_init_es_entry :=
+  match goal with
+  | |- context [PathMap.get ?p init_es] =>
+      let obj' := eval cbv-[am_ge Tofino.extern_match] in
+        (PathMap.get p init_es) in
+      change (PathMap.get p init_es) with obj'
+  end.
+
+Lemma init_es_reg_repr :
+  @Some (extern_object)
+    (Tofino.ObjRegister
+       (Tofino.new_register 262144
+          (ValBaseBit [false; false; false; false; false; false; false; false]))) =
+  Some
+    (Tofino.ObjRegister (map FilterRepr.bool_to_val (` (ConFilter.row_empty H_num_slots)))).
+Proof.
+  Transparent Tofino.new_register.
+  unfold Tofino.new_register.
+  Opaque Tofino.new_register.
+  unfold ConFilter.row_empty, proj1_sig.
+  rewrite map_Zrepeat.
+  f_equal.
+Qed.
+
+Lemma filter_repr_empty_init_es : forall t,
+  filter_repr (empty t) init_es.
+Proof.
+  intros.
+  unfold filter_repr; hnf.
+  exists filter_empty.
+  split.
+  { repeat first [
+      apply conj; hnf
+    | apply I
+    ];
+    try simpl_init_es_entry;
+    try apply init_es_reg_repr.
+    - exists 0.
+      repeat first [
+        apply conj; hnf
+      | apply I
+      ].
+      + simpl_init_es_entry.
+        reflexivity.
+      + reflexivity.
+    - simpl. inversion 1.
+    - auto.
+    - reflexivity.
+  }
+  hnf.
+  apply AbsFilter.filter_sim_empty;
+    resolve_parameter_conditions.
+Qed.
+
+Print property.
+
 Theorem main_theorem : forall h p es' rs' res,
   process_packets ge P4_types.metadata_t init_es (h ++ [p]) es' (rs' ++ [res]) ->
+  abs_flow_wf (h ++ [p]) ->
   valid_flow (h ++ [p]) ->
   property h p res.
 Proof.
   intros.
   eapply process_packets_trans_fw with (f := empty (get_tstamp (Znth 0 (h++[p])))) in H.
-  2 : { admit. }
+  3 : auto.
+  2 : apply filter_repr_empty_init_es.
   eapply flow_level_property; auto.
   apply <- high_level_exec_trans_fw_iff.
   destruct H. destruct H.
   eauto.
-Admitted.
+Qed.
